
$$\mathcal{I} = \int_{-\pi}^{\pi}dk \frac{\gamma^2sin^2k}{((h-cosk)^2+\gamma^2sin^2k)^2} \to e^{ik}=z; \ \frac{dz}{iz}=dk$$
$$\mathcal{I} = \gamma^2\oint \frac{dz}{iz} \frac{(-\frac{1}{4}) (z-\frac{1}{z})^2}{((h-\frac{1}{2}(z+\frac{1}{z}))^2-\frac{\gamma^2}{4}(z-\frac{1}{z})^2)^2} = (-\frac{\gamma^2}{4}) \oint \frac{dz}{iz} \frac{(z-\frac{1}{z})^2}{((h-\frac{1}{2}(z+\frac{1}{z})+\frac{\gamma}{2}(z-\frac{1}{z}))(h-\frac{1}{2}(z+\frac{1}{z})-\frac{\gamma}{2}(z-\frac{1}{z})))^2}$$
$$ =(-\frac{\gamma^2}{4}) \oint \frac{dz}{iz} \frac{(z^2-1)^2}{((hz-\frac{1}{2}(z^2+1)+\frac{\gamma}{2}(z^2-1))(hz-\frac{1}{2}(z^2+1)-\frac{\gamma}{2}(z^2-1)))^2}$$
$$=(-\gamma^2) \oint \frac{dz}{iz} \frac{(z^2-1)^2}{((2hz-(z^2+1)+\gamma(z^2-1))(2hz-(z^2+1)-\gamma(z^2-1)))^2}$$
$$$$
$$g_1(z) = z^2(\gamma-1)+2hz-(\gamma+1) \implies Poles: \ \ \  z_1^{\pm}=\frac{-h \pm\sqrt{h^2+\gamma^2 -1}}{(\gamma-1)} $$



$$g_2(z)= z^2(\gamma+1)-2hz-(\gamma-1) \implies Poles: \ \ \  z_2^{\pm} =\frac{h \pm \sqrt{h^2+\gamma^2-1}}{(\gamma+1)}$$


Say 
$$|z_1^+| =|\frac{-h +\sqrt{h^2+\gamma^2 -1}}{(\gamma-1)}|<1  \implies h^2 + (h^2+\gamma^2-1) - 2h\sqrt{h^2+\gamma^2-1} < (\gamma - 1)^2=\gamma^2+1-2\gamma$$
$$\implies h(h- \sqrt{h^2+\gamma^2-1}) < (1-\gamma) \implies -\sqrt{h^2+\gamma^2-1} < \frac{(1-\gamma)}{h}-h \implies h^2 + \gamma^2 - 1 < \frac{1}{h}(1+\gamma^2-2\gamma - h^2)$$
$$f_1(x, y) = \frac{-x +\sqrt{x^2+y^2 -1}}{(y-1)}$$
$$\sum^{\infty}_{n=0}\frac{x^n}{n \times n!}$$

$$\  |z_2^{+}| = | \ \frac{h +\sqrt{h^2+\gamma^2 -1}}{(\gamma+1)} \ | \ \leq \  1 $$